kmsidentifier internal error due to no witness after subset

KmsArnIdentifier.dfy
@@ -1,10 +1,10 @@
+
 predicate ArnString?(s: string)
 {
     s == "arn"
 }
 // MUST start with string arn
-type ArnString = s:string | ArnString?(s) witness "arn"
-
+type ArnString = s:string |  s == "arn" witness *
 
 
 // The partition MUST be a non-empty
@@ -32,11 +32,14 @@ predicate RegionString?(s:string)
 type RegionString = s:string | RegionString?(s) witness *
 
 //The account MUST be a non-empty string
+
+
 predicate AccountString?(s:string)
 {
     |s|!=0
 
 }
+
 type AccountString = s:string | AccountString?(s) witness *
 
 
@@ -50,6 +53,10 @@ predicate KmsResource?(x:string, y:string)
     (x=="alias" ||x == "key") && |y| != 0
 }
 
+datatype Resource = Resource(
+    rtype : string,
+    id : string
+)
 
 datatype ARN = ARN(
     arnLiteral: string,
@@ -62,75 +69,103 @@ datatype ARN = ARN(
 
 
 
-// type KmsArn = a: ARN | KmsArn?(a) witness *
 
 
-type resourceType = s:string | s == "alias" || s == "key" witness *
+type ResourceType = s:string | s == "alias" || s == "key" witness *
 
 type ResourceId = s:string | |s| != 0 witness *
 
 
 
-datatype Resource = Resource(
-    rtype : string,
-    id : string
-)
-
 datatype KmsResource = KmsResource(
-    rtype : resourceType,
+    rtype : ResourceType,
     id : ResourceId
 )
+
+//remeber to add witness
+type KeyType = s:ResourceType | s == "key" 
+type MrkId = s:ResourceId | |s|>4 && s[..4] == "mrk-" witness*
+
+predicate MrkId? (s:ResourceId)
+{
+    |s|>4 && s[..4] == "mrk-"
+}
+
+predicate KeyType?(s:ResourceType)
+{
+    s == "key" 
+}
+
+datatype MrkResource = MrkResource(
+    rtype : KeyType,
+    id : MrkId
+
+)
+
+predicate AwsKmsMrkIdentifier(a:KmsArnSubtype)
+{
+    true
+    // && KeyType?(a.resource.rtype)
+    // && MrkId?(a.resource.id)
+}
+
+type KmsArnSubtype = a: ARN | KmsArn?(a) witness *
+
+
 
 datatype KmsArnDatatype = KmsArnDatatype(
     arnLiteral: ArnString,
     partition: PartitionString,
     service: ServiceString,
     region: RegionString,
-    account: AccountString,
-    resource: KmsResource
+    account: AccountString
+    // resource: KmsResource
 )
 
-
-
-
-// predicate KmsArn?(a:ARN)
-
+// lemma asdf(stuff: seq<string>)
+//     requires 5 == |stuff|
 // {
-//     if
-//         // MUST start with string arn
-//         && a.arnLiteral == "arn"
-
-//         // The partition MUST be a non-empty
-//         && |a.partition| !=0
-
-//         // The service MUST be the string kms
-//         && a.service == "kms"
-
-//         //The account MUST be a non-empty string
-//         && |a.account| != 0
-
-//         // The region MUST be a non-empty string
-//         && |a.region| !=0
-
-//         // then it leads to resource type to be key or alias, and both id cannot be empty
-//         &&  |a.resource|>=2
-//         &&  (
-//             (&& a.resource[0] == "key"
-//             && |a.resource[1]|!=0 ) 
-//             || 
-//             (&& a.resource[0] == "alias" 
-//             && |a.resource[1]| != 0 )
-//             )
-//     then true
-//     else false
+//     var k := KmsArnDatatype( stuff[0], stuff[1], stuff[2], stuff[3], stuff[4]);
 // }
 
-// method test()
-// {
-//     assert ARN("arn","aws","kms","us-east-1","2222222222222",["key","testid"]).ARN? == true;
 
-//     assert KmsArn?(ARN("arn","aws","kms","us-east-1","2222222222222",["alias","testid"])) == true;
+predicate KmsArn?(a:ARN)
 
-//     assert KmsArnDatatype("arn","aws","kms","us-east-1","2222222222222",["key","testid"]).KmsArnDatatype? == true;
+{
+    // MUST start with string arn
+    && a.arnLiteral == "arn"
 
-// }
+    // The partition MUST be a non-empty
+    && |a.partition| !=0
+
+    // The service MUST be the string kms
+    && a.service == "kms"
+
+    //The account MUST be a non-empty string
+    && |a.account| != 0
+
+    // The region MUST be a non-empty string
+    && |a.region| !=0
+
+    // then it leads to resource type to be key or alias, and both id cannot be empty
+    &&  (
+        (&& a.resource.rtype == "key"
+        && |a.resource.id| != 0 ) 
+        || 
+        (&& a.resource.rtype == "alias" 
+        && |a.resource.id| != 0 )
+        )
+
+}
+
+method test()
+{
+    // assert ARN("arn","aws","kms","us-east-1","2222222222222",Resource("key","test")).ARN? == false;
+
+    // assert KmsArn?(ARN("arn","aws","kms","us-east-1","2222222222222",Resource("key","test"))) == true;
+
+    // assert (KmsArnDatatype("arn","aws","kms","us-east-1","2222222222222",KmsResource("key","test")).KmsArnDatatype?) == false;
+
+    // assert AwsKmsMrkIdentifier(KmsArnDatatype("arn","aws","kms","us-east-1","2222222222222",KmsResource("key","test"))) == false;
+
+}
