KmsArnIdeGen3.dfy
@@ -1,0 +1,68 @@
+predicate ArnString?(s: string)
+{
+    s == "arn"
+}
+// MUST start with string arn
+type ArnString = s:string |  s == "arn" witness *
+
+
+// The partition MUST be a non-empty
+predicate PartitionString?(s:string)
+{
+    s != ""
+}
+type PartitionString = s:string | PartitionString?(s) witness *
+
+
+
+// The service MUST be the string kms
+predicate ServiceString?(s:string)
+{
+    s == "kms"
+}
+
+type ServiceString = s | ServiceString?(s) witness *
+
+// The region MUST be a non-empty string
+predicate RegionString?(s:string)
+{
+    |s|!=0
+}
+type RegionString = s:string | RegionString?(s) witness *
+
+//The account MUST be a non-empty string
+
+
+predicate AccountString?(s:string)
+{
+    |s|!=0
+
+}
+
+type AccountString = s:string | AccountString?(s) witness *
+
+
+// The resource section MUST be non-empty and MUST be split by a single / any additional / are included in the resource id
+// The resource type MUST be either alias or key
+// The resource id MUST be a non-empty string 
+// this seq<string> length is 2, x[0] is key, x[1] is ID.
+
+predicate KmsResource?(x:string, y:string)
+{
+    (x=="alias" ||x == "key") && |y| != 0
+}
+
+datatype Resource = Resource(
+    rtype : string,
+    id : string
+)
+
+datatype ARN = ARN(
+    arnLiteral: string,
+    partition: string,
+    service: string,
+    region: string,
+    account: string,
+    resource: Resource
+)
+
