test.dfy
@@ -1,0 +1,63 @@
+//Failure compatible types
+
+
+datatype Result<T> =
+| Success(value: T)
+| Failure(error: string)
+{
+  predicate method IsFailure() {
+    this.Failure?
+  }
+  function method PropagateFailure<U>(): Result<U>
+    requires IsFailure()
+  {
+    Failure(this.error) // this is Result<U>.Failure(...)
+  }
+
+  function method Extract(): T
+    requires !IsFailure()
+  {
+    this.value
+  }
+
+}
+
+function method split(s:string) :(output: seq<string>)
+
+function method F(s:string): Result<seq<string>>
+{
+    var test := split(s);
+
+    if (|test| == 5) then
+        Result.Success(test)
+    else
+        Result.Failure("did not split to 5")
+}
+
+datatype ARN = ARN(
+    l: string,
+    p: string,
+    s: string,
+    a: string,
+    r: string
+)
+
+function method use(s: string): Result<string>
+
+{
+    var asdf :- F(s);
+
+    // var t := F(s);
+
+    // if t.Failure? then
+    //     Failure(t.error)
+    // else
+    //     var v := t.value;
+
+    // var asdf := F(s);
+    // var asdf := split(s);
+
+    // Success(ARN(asdf[0], asdf[1], asdf[2], asdf[3], asdf[4])) 
+    Failure("hahahah")
+}
+
